Get StreamingImpl to at least resolve

TestModels/dafny-dependencies/StandardLibrary/src/Streams.dfy
@@ -26,10 +26,13 @@ module {:options "--function-syntax:4"} StandardLibrary.Streams {
       Flatten(Enumerated(Outputs(history)))
     }
 
-    function ContentLength(): (res: Option<uint64>)
+    // TODO: This should be an Option<uint64>, 
+    // but that ends up running into a conflict
+    // when trying to import Wrappers and Std.Wrappers at the same time.
+    function ContentLength(): (res: uint64)
       requires Valid()
       reads this, Repr
-      ensures res.Some? ==> res.value as int == |data|
+      ensures res as int == |data|
 
     ghost predicate CanProduce(history: seq<((), Option<bytes>)>)
       decreases height
@@ -87,10 +90,10 @@ module {:options "--function-syntax:4"} StandardLibrary.Streams {
   /*
    * Wraps an Enumerator up as a non-rewindable DataStream.
    */
-  class EnumeratorDataStream<bytes> extends DataStream {
+  class EnumeratorDataStream extends DataStream {
 
     const wrapped: Enumerator<BoundedInts.bytes>
-    const length: Option<uint64>
+    const length: uint64
 
     ghost predicate Valid() 
       reads this, Repr 
@@ -102,7 +105,7 @@ module {:options "--function-syntax:4"} StandardLibrary.Streams {
       && ValidComponent(wrapped)
       && CanProduce(history)
       && |data| <= UINT64_MAX as int
-      && (length.Some? ==> length.value as int == |data|)
+      && length as int == |data|
     }
 
     lemma {:axiom} ProducesTerminated(history: seq<((), Option<BoundedInts.bytes>)>)
@@ -114,11 +117,11 @@ module {:options "--function-syntax:4"} StandardLibrary.Streams {
       wrapped.Limit()
     }
 
-    constructor(wrapped: Enumerator<BoundedInts.bytes>, length: Option<uint64>, ghost data: BoundedInts.bytes) 
+    constructor(wrapped: Enumerator<BoundedInts.bytes>, length: uint64, ghost data: BoundedInts.bytes) 
       requires wrapped.Valid()
       requires wrapped.history == []
       requires |data| <= UINT64_MAX as int
-      requires length.Some? ==> length.value as int == |data|
+      requires length as int == |data|
       ensures Valid()
     {
       this.wrapped := wrapped;
@@ -130,10 +133,10 @@ module {:options "--function-syntax:4"} StandardLibrary.Streams {
       this.height := wrapped.height + 1;
     }
 
-    function ContentLength(): (res: Option<uint64>)
+    function ContentLength(): (res: uint64)
       requires Valid()
       reads this, Repr
-      ensures res.Some? ==> res.value as int == |data|
+      ensures res as int == |data|
     {
       length
     }
@@ -229,12 +232,12 @@ module {:options "--function-syntax:4"} StandardLibrary.Streams {
       this.height := 1;
     }
 
-    function ContentLength(): (res: Option<uint64>)
+    function ContentLength(): (res: uint64)
       requires Valid()
       reads this, Repr
-      ensures res.Some? ==> res.value as int == |data|
+      ensures res as int == |data|
     {
-      Some(|s| as uint64)
+      |s| as uint64
     }
 
     predicate Rewindable()
